Some more preliminary work

src/Decide.v
@@ -20,17 +20,93 @@ Generalizable All Variables.
 
 Section Decide.
 
+Program Definition Term_Category {C objs arrs} : Category := {|
+  obj := obj_idx;
+  hom := fun x y => ∃ f f', @term_denote C objs arrs x y f = Some f';
+  homset := fun x y => {| equiv := fun f g => `1 `2 f ≈ `1 `2 g |};
+  id := fun x => (Identity x; (@id C (objs x); _));
+  compose := fun x y z f g => (Compose y `1 f `1 g; (`1 `2 f ∘ `1 `2 g; _))
+|}.
+Next Obligation. now equalities. Defined.
+Next Obligation. now rewrite X2, X0. Defined.
+
+Program Definition Term_Category' {C objs arrs} : Category := {|
+  obj := obj_idx;
+  hom := fun _ _ => Term;
+  homset := fun x y => {| equiv := fun f g =>
+    @term_denote C objs arrs x y f ≈ @term_denote C objs arrs x y g |};
+  id := Identity;
+  compose := fun _ y _ => Compose y
+|}.
+Next Obligation.
+  equivalence.
+  - destruct (term_denote objs arrs x y x0) eqn:?; auto.
+    reflexivity.
+  - destruct (term_denote objs arrs x y x0) eqn:?;
+    destruct (term_denote objs arrs x y y0) eqn:?; auto.
+    now symmetry.
+  - destruct (term_denote objs arrs x y x0) eqn:?;
+    destruct (term_denote objs arrs x y y0) eqn:?;
+    destruct (term_denote objs arrs x y z) eqn:?; auto.
+      now transitivity h0.
+    contradiction.
+Defined.
+Next Obligation.
+  proper.
+  destruct (term_denote objs arrs y z x0) eqn:?;
+  destruct (term_denote objs arrs x y x1) eqn:?;
+  destruct (term_denote objs arrs y z y0) eqn:?;
+  destruct (term_denote objs arrs x y y1) eqn:?; auto.
+  now rewrite X, X0.
+Defined.
+Next Obligation.
+  equalities'; auto.
+  equalities.
+  destruct (term_denote objs arrs x y f) eqn:?; cat.
+Qed.
+Next Obligation.
+  equalities'; auto.
+  equalities.
+  destruct (term_denote objs arrs x y f) eqn:?; cat.
+Qed.
+Next Obligation.
+  destruct (term_denote objs arrs z w f) eqn:?;
+  destruct (term_denote objs arrs y z g) eqn:?;
+  destruct (term_denote objs arrs x y h) eqn:?; cat.
+Qed.
+Next Obligation.
+  destruct (term_denote objs arrs z w f) eqn:?;
+  destruct (term_denote objs arrs y z g) eqn:?;
+  destruct (term_denote objs arrs x y h) eqn:?; cat.
+Qed.
+
+Existing Instance Term_Category'.
+
+Lemma term_denote_append C objs arrs x m y (f1 : Term) :
+  (f1 : @hom (@Term_Category' C objs arrs) x y) ≈ term_append f1 (Identity m).
+Proof.
+  simpl.
+  generalize dependent y.
+  generalize dependent m.
+  generalize dependent x.
+  induction f1; simpl; intros; equalities.
+  - reflexivity.
+  - destruct (arrs _) eqn:?; auto.
+    destruct s, s; equalities.
+    equalities'; auto.
+    equalities'; auto.
+    equalities; reflexivity.
+  - specialize (IHf1_1 m m y).
+    destruct (term_denote objs arrs m y f1_1) eqn:?;
+    destruct (term_denote objs arrs m y (term_append f1_1 (Identity m))) eqn:?.
+Admitted.
+
 Lemma term_denote_term_append C objs arrs x m y f1 f2 f' g' :
   term_denote objs arrs m y (term_append f1 (Identity m)) ≈ Some f' ->
   term_denote objs arrs x m (term_append f2 (Identity x)) ≈ Some g' ->
   @term_denote C objs arrs x y (term_append (Compose m f1 f2) (Identity x)) ≈ Some (f' ∘ g').
 Proof.
   simpl; intros.
-  destruct (term_append f2 (Identity x)); simpl in *.
-  - repeat equalities; simpl_eq.
-    admit.
-  - admit.
-  - simpl.
 Admitted.
 
 Lemma normalize_equiv C objs arrs x y f f' :
